Add Sprint.lean and update Runner.lean to match
This completes the trace/sprint refactoring. Previously, sprints were
defined in Runner.lean and included logic for following the y-axis
and stopping before the angel's maximum range was exceeded. However,
the final steps of Mathe's proof require us to consider the runner's
behavior when one or both of these limits is removed.

With the refactored code, a "trace" is the path taken by the runner
for a given starting point, length, and list of blocked cells.
A "sprint" is then defined as a trace which respects the angel's range.
Finally, the function "make_run" assembles a sequence of sprints which
begins at (0, 0) and defines the list of blocked cells such that the
runner never steps on an eaten cell or crosses the y-axis.

AngelDevil/Runner.lean
@@ -4,6 +4,8 @@ import AngelDevil.Defs
 import AngelDevil.Basic
 import AngelDevil.Append
 import AngelDevil.Nice
+import AngelDevil.Sprint
+import AngelDevil.Bound
 
 set_option linter.style.longLine false
 
@@ -12,25 +14,6 @@ set_option linter.style.longLine false
    time they are blocked by a cell the Devil has eaten.
 -/
 
-@[ext] structure RunState where
-  x : Int -- Current location, x-coord
-  y : Int -- Current location, y-coord
-  u : Int -- Direction of travel, x-coord
-  v : Int -- Direction of travel, y-coord
-  unit : u * u + v * v = 1 -- ⟨u, v⟩ should be a unit vector
-
--- Prove that we can determine whether two 'RunState' are equal
-instance : DecidableEq RunState := fun a b ↦
-  if h : a.x = b.x ∧ a.y = b.y ∧ a.u = b.u ∧ a.v = b.v then
-    isTrue (RunState.ext_iff.mpr h)
-  else
-    isFalse (fun h' ↦ h (RunState.ext_iff.mp h'))
-
--- Convenience macros for repackaging the location and direction
--- parameters as Int × Int
-def loc (rs : RunState) : Int × Int := ⟨rs.x, rs.y⟩
-def dir (rs : RunState) : Int × Int := ⟨rs.u, rs.v⟩
-
 -- The runner begins at the origin, running northward (up the positive y-axis)
 def run_start : RunState where
   x := 0
@@ -38,231 +21,6 @@ def run_start : RunState where
   u := 0
   v := 1
   unit := by simp
-
-/- Move forward one cell, turn left, and move forward one cell again.
-   Note that for the purposes of counting traversed walls, this counts
-   as a single step, not two. -/
-def turn_left (rs : RunState) : RunState where
-  x := rs.x + rs.u - rs.v
-  y := rs.y + rs.u + rs.v
-  u := -rs.v
-  v := rs.u
-  unit := by
-    rw [Int.neg_mul_neg, Int.add_comm]
-    exact rs.unit
-
--- Move forward one cell
-def move_forward (rs : RunState) : RunState where
-  x := rs.x + rs.u
-  y := rs.y + rs.v
-  u := rs.u
-  v := rs.v
-  unit := rs.unit
-
--- Without changing cells, turn 90-degrees to the right
-def turn_right (rs : RunState) : RunState where
-  x := rs.x
-  y := rs.y
-  u := rs.v
-  v := -rs.u
-  unit := by
-    rw [Int.neg_mul_neg, Int.add_comm]
-    exact rs.unit
-
--- Turning right doesn't change the location, only the direction
-lemma turn_right_loc (rs : RunState) : loc (turn_right rs) = loc rs := rfl
-
-abbrev blocked (eaten : List (Int × Int)) (x : Int × Int) :=
-  x.1 < 0 ∨ x ∈ eaten
-
-/- Determine where the next step of the run would take us.
-   That is, try each of the actions listed above (turn left, move forward,
-   and turn right) and pick the first which lands on an unblocked cell
--/
-def next_step (eaten : List (Int × Int)) (rs : RunState) : RunState :=
-  if ¬blocked eaten (loc (turn_left rs)) then turn_left rs else
-  if ¬blocked eaten (loc (move_forward rs)) then move_forward rs else
-  turn_right rs
-
-/- Attempts to add 'rs' to the current partial sprint.
-   If it succeeds, repeat with the cell indicated by 'next_step'.
--/
-def sprint_partial (p ns : Nat) (start : Int × Int) (eaten : List (Int × Int)) (rs : RunState) : List RunState :=
-  if hterm : 2 * p < ns ∨ ¬close p start (loc rs) then [] else
-  rs :: (sprint_partial p (ns + 1) start eaten (next_step eaten rs))
-termination_by 2 * p + 1 - ns
-decreasing_by
-  push_neg at hterm
-  rw [add_comm ns, Nat.sub_add_eq, Nat.add_one_sub_one, Nat.sub_add_comm hterm.1]
-  exact Nat.lt_add_one_of_le (le_refl _)
-
--- If the list constructed by 'sprint_partial' is not empty, the first element of the list will be 'rs'
-lemma sprint_partial_getElem_zero_of_nonnil (p ns : Nat) (start : Int × Int) (eaten : List (Int × Int)) (rs : RunState) :
-  (hnnil : sprint_partial p ns start eaten rs ≠ []) →
-  (sprint_partial p ns start eaten rs)[0]'(List.length_pos_iff.mpr hnnil) = rs := by
-  intro hnnil
-  -- Use the trick of starting with 'sprint_partial = sprint_partial' followed by 'nth_rw'
-  -- to expand only the right-hand side. This allows us to easily do
-  -- the necessary rewrites without having to worry about 'getElem_congr_coll'
-  have : sprint_partial p ns start eaten rs = _ := rfl
-  nth_rw 2 [sprint_partial] at this
-  by_cases hterm : ns > 2 * p ∨ ¬close p start (loc rs)
-  · -- If we hit the termination case this leads to a contradiction
-    rw [dif_pos hterm] at this
-    exact False.elim (hnnil this)
-  rw [dif_neg hterm] at this
-  rw [getElem_congr_coll this, List.getElem_cons_zero]
-
--- If the list constructed by 'sprint_partial' is not empty, ns < 2 * p + 1
-lemma sprint_partial_nslt_of_nonnil (p ns : Nat) (start : Int × Int) (eaten : List (Int × Int)) (rs : RunState) :
-  (hnnil : sprint_partial p ns start eaten rs ≠ []) → ns < 2 * p + 1 := by
-  intro hnnil
-  apply Nat.lt_add_one_of_le
-  contrapose! hnnil
-  rename' hnnil => ltns
-  unfold sprint_partial
-  rw [dif_pos (Or.inl ltns)]
-
--- If the list constructed by 'sprint_partial' is not empty, then the first element is close to 'start'
-lemma sprint_partial_close_getElem_zero_of_nonnil (p ns : Nat) (start : Int × Int) (eaten : List (Int × Int)) (rs : RunState) :
-  (hnnil : sprint_partial p ns start eaten rs ≠ []) →
-  close p start (loc ((sprint_partial p ns start eaten rs)[0]'(List.length_pos_iff.mpr hnnil))) := by
-  intro hnnil
-  rw [sprint_partial_getElem_zero_of_nonnil]
-  · contrapose! hnnil
-    rename' hnnil => hnclose
-    unfold sprint_partial
-    rw [dif_pos (Or.inr hnclose)]
-  · assumption
-
--- If the list constructed by 'sprint_partial' is not empty, rewrite it in 'cons' form.
-lemma sprint_partial_cons_of_nonnil (p ns : Nat) (start : Int × Int) (eaten : List (Int × Int)) (rs : RunState) :
-  (hnnil : sprint_partial p ns start eaten rs ≠ []) →
-  sprint_partial p ns start eaten rs = (rs :: (sprint_partial p (ns + 1) start eaten (next_step eaten rs))) := by
-  intro hnnil
-  nth_rw 1 [sprint_partial]
-  split_ifs with hterm
-  · apply hnnil
-    unfold sprint_partial
-    rw [dif_pos hterm]
-  · rfl
-
--- Any element of a partial sprint is close to the start of the sprint
-lemma sprint_partial_mem_close (p ns : Nat) (start : Int × Int) (eaten : List (Int × Int)) (rs : RunState) :
-  ∀ x ∈ sprint_partial p ns start eaten rs, close p start (loc x) := by
-  intro x hxmem
-  rcases List.getElem_of_mem hxmem with ⟨i, ilt, helem⟩
-  by_cases iz : i = 0
-  · -- We've already proven that if 'sprint_partial ≠ []', sprint_partial[0] is "close"
-    subst iz
-    subst helem
-    apply sprint_partial_close_getElem_zero_of_nonnil
-    exact List.ne_nil_of_mem hxmem
-  · rename' iz => inz; push_neg at inz
-    -- Otherwise, rewrite the list in 'cons' form and use recursion to close the goal
-    rw [getElem_congr_coll (sprint_partial_cons_of_nonnil p ns start eaten rs (List.ne_nil_of_mem hxmem))] at helem
-    rw [getElem_congr_idx ((Nat.sub_one_add_one inz).symm), List.getElem_cons_succ] at helem
-    exact sprint_partial_mem_close _ _ _ _ _ x (List.mem_of_getElem helem)
-termination_by (2 * p + 1 - ns)
-decreasing_by
-  have hnnil : sprint_partial p ns start eaten rs ≠ [] :=
-    List.ne_nil_of_length_pos (lt_of_le_of_lt (Nat.zero_le _) ilt)
-  have nsle : ns ≤ 2 * p := by
-    apply Nat.le_of_lt_add_one
-    apply sprint_partial_nslt_of_nonnil
-    exact hnnil
-  rw [add_comm ns, Nat.sub_add_eq, Nat.add_one_sub_one, Nat.sub_add_comm nsle]
-  exact Nat.lt_add_one_of_le (le_refl _)
-
--- Prove that a partial sprint never steps on an eaten cell
-lemma sprint_partial_avoids_eaten (p ns : Nat) (start : Int × Int)
-  (eaten : List (Int × Int)) (rs : RunState) (hsafe : loc rs ∉ eaten) :
-  ∀ x ∈ sprint_partial p ns start eaten rs, loc x ∉ eaten := by
-  intro x hmem₀ hmem₁
-  unfold sprint_partial at hmem₀
-  split_ifs at hmem₀ with h₀
-  · exact (List.mem_nil_iff _).mp hmem₀
-  push_neg at h₀
-  rcases List.mem_cons.mp hmem₀ with lhs | rhs
-  · subst lhs; contradiction
-  -- This next part is the most technical:
-  -- We have to go through each of the advancement cases and
-  -- show that we never step on an eaten cell
-  have hsafe' : loc (next_step eaten rs) ∉ eaten := by
-    intro hmem₂
-    unfold next_step at hmem₂
-    split_ifs at hmem₂ with h₁ h₂
-    · rw [turn_right_loc] at hmem₂
-      contradiction
-    · unfold blocked at h₂
-      push_neg at h₂
-      exact h₂.2 hmem₂
-    · unfold blocked at h₁
-      push_neg at h₁
-      exact h₁.2 hmem₂
-  exact sprint_partial_avoids_eaten p (ns + 1) start eaten (next_step eaten rs) hsafe' x rhs hmem₁
-termination_by 2 * p + 1 - ns
-decreasing_by
-  rw [Nat.sub_add_eq]
-  apply Nat.sub_one_lt (Nat.sub_ne_zero_of_lt (Nat.lt_add_one_of_le _))
-  push_neg at h₀
-  exact h₀.1
-
--- A sprint is a sequence of steps taken by the runner between moves by the devil.
--- Later we will show that the cells corresponding to the beginning and end of
--- the sprints can be used to construct an angel which escapes the Nice Devil.
-def sprint (p : Nat) (rs₀ : RunState) (eaten : List (Int × Int)) : List RunState :=
-  sprint_partial p 0 (loc rs₀) eaten rs₀
-
--- If 'p' is positive, the sprint will not be empty
--- Up to this point we have not needed this assumption, but it appears
--- to be necessary if we wish to match the logic of the original paper.
-lemma sprint_nonnil_of_ppos (p : Nat) (rs₀ : RunState) (eaten : List (Int × Int)) :
-  0 < p → sprint p rs₀ eaten ≠ [] := by
-  intro hpos
-  unfold sprint sprint_partial
-  split_ifs with hterm
-  · contrapose! hterm
-    constructor
-    · linarith
-    · exact close_self p (loc rs₀)
-  exact List.cons_ne_nil _ _
-
-lemma sprint_getElem_zero_of_ppos (p : Nat) (rs₀ : RunState) (eaten : List (Int × Int)) :
-  (ppos : 0 < p) → (sprint p rs₀ eaten)[0]'(by
-    apply List.length_pos_of_ne_nil
-    exact sprint_nonnil_of_ppos p rs₀ eaten ppos
-  ) = rs₀ :=
-  fun ppos ↦ sprint_partial_getElem_zero_of_nonnil p 0 (loc rs₀) eaten rs₀
-    (sprint_nonnil_of_ppos p rs₀ eaten ppos)
-
--- All run states in a sprint are close to the start of that sprint
-lemma sprint_close_mem_head (p : Nat) (hpos : 0 < p) (rs₀ : RunState) (eaten : List (Int × Int)) :
-  ∀ x ∈ (sprint p rs₀ eaten), close p (loc x)
-  (loc ((sprint p rs₀ eaten).head (sprint_nonnil_of_ppos p rs₀ eaten hpos))) := by
-  intro x xmem
-  have hnnil := sprint_nonnil_of_ppos p rs₀ eaten hpos
-  unfold sprint at *
-  rw [close_comm]
-  convert sprint_partial_mem_close p 0 (loc rs₀) eaten rs₀ x xmem
-  rwa [List.head_eq_getElem_zero hnnil, sprint_partial_getElem_zero_of_nonnil]
-
--- Prove that the first and last cells in a sprint are "close"
-lemma sprint_close_first_last (p : Nat) (hpos : 0 < p) (rs₀ : RunState) (eaten : List (Int × Int)) :
-  close p
-  (loc ((sprint p rs₀ eaten).head (sprint_nonnil_of_ppos p rs₀ eaten hpos)))
-  (loc ((sprint p rs₀ eaten).getLast (sprint_nonnil_of_ppos p rs₀ eaten hpos))) := by
-  have hnnil := sprint_nonnil_of_ppos p rs₀ eaten hpos
-  rw [close_comm]
-  exact sprint_close_mem_head p hpos rs₀ eaten _ (List.getLast_mem hnnil)
-
--- The runner never visits an eaten cell
--- (as long as they don't start on an eaten cell)
-lemma sprint_avoids_eaten (p : Nat) (rs₀ : RunState)
-  (eaten : List (Int × Int)) (hsafe : loc rs₀ ∉ eaten) :
-  ∀ x, x ∈ (sprint p rs₀ eaten) → loc x ∉ eaten :=
-  fun x smem emem ↦
-  sprint_partial_avoids_eaten p 0 (loc rs₀) eaten rs₀ hsafe x smem emem
 
 /- The three different structures needed to define the runner's journey
    have interdependencies that make them difficult to construct separately.
@@ -297,6 +55,13 @@ lemma final_state_of_sprints_nil {p : Nat} (S : RunBuilder p) (hnil : S.sprints 
   unfold final_state
   rw [dif_pos (List.length_eq_zero_iff.mpr hnil)]
 
+-- If 'sprints' is nonnil, the final state is an element in the final sprint
+lemma final_state_getLast_mem_of_nonnil {p : Nat} (S : RunBuilder p) (hnil : S.sprints ≠ []) :
+  final_state S ∈ S.sprints.getLast hnil := by
+  unfold final_state
+  rw [dif_neg (Nat.ne_zero_of_lt (List.length_pos_of_ne_nil hnil))]
+  apply List.getLast_mem
+
 -- The location given by 'final_state' matches the last cell in the builder journey
 lemma final_state_loc_eq_journey_last {p : Nat} (S : RunBuilder p) :
   loc (final_state S) = last S.A := by
@@ -306,9 +71,33 @@ lemma final_state_loc_eq_journey_last {p : Nat} (S : RunBuilder p) :
   · push_neg at hlz
     exact S.dest (List.ne_nil_of_length_pos (Nat.pos_of_ne_zero hlz))
 
+-- List of cells necessary to prevent the runner from ever moving west of the y-axis
+def west_wall (p n : Nat) :=
+  List.map (fun i : Nat ↦ (-1, (i : Int))) (List.range (p * n + 1))
+
+-- Any cell which is an elment of the west wall has x-coordinate -1
+lemma west_wall_xcoord_of_mem (p n : Nat) :
+  ∀ l ∈ west_wall p n, l.1 = -1 := by
+  unfold west_wall
+  intro l lmem
+  rcases List.getElem_of_mem lmem with ⟨i, ilt, hi⟩
+  rw [List.getElem_map] at hi
+  rw [← hi]
+
+-- Prove the conditions for a cell to be an element of the west wall
+lemma west_wall_mem (p n : Nat) :
+  ∀ i (_ : i ≤ p * n), (-1, Int.ofNat i) ∈ west_wall p n := by
+  intro i ile
+  unfold west_wall
+  apply List.mem_iff_getElem.mpr
+  use i, (by rw [List.length_map, List.length_range]; exact Nat.lt_add_one_of_le ile)
+  rw [List.getElem_map, List.getElem_range]; rfl
+
 -- Get the next sprint to be added to the builder
+-- Note that for the purposes of finding the next sprint, a wall of cells
+-- is added along the y-axis that prevent the runner from ever moving that direction.
 def next_sprint {p : Nat} (S : RunBuilder p) : List RunState :=
-  sprint p (final_state S) S.eaten
+  sprint p (final_state S) (List.union S.eaten (west_wall p S.eaten.length))
 
 lemma next_sprint_nonnil {p : Nat} (S : RunBuilder p) :
   next_sprint S ≠ [] := by
@@ -320,7 +109,7 @@ lemma next_sprint_nonnil {p : Nat} (S : RunBuilder p) :
 lemma next_sprint_first_eq_builder_last {p : Nat} (S : RunBuilder p) :
   final_state S = (next_sprint S)[0]'(by
     apply List.length_pos_of_ne_nil
-    exact sprint_nonnil_of_ppos p (final_state S) S.eaten S.ppos
+    exact sprint_nonnil_of_ppos p (final_state S) _ S.ppos
   ) := by
   unfold next_sprint
   rw [sprint_getElem_zero_of_ppos]
@@ -383,7 +172,7 @@ lemma list_singleton_ne_nil {α : Type} (x : α) : [x] ≠ [] := by
   norm_num
 
 /- Add another sprint to a 'RunBuilder'
-   Original this was named 'make_run' and used recursion to
+   Originally this was named 'make_run' and used recursion to
    directly construct the RunBuilder (rather than taking 'S' as an argument).
    Unfortunately this caused timeouts, so now 'make_run' handles the recursion
    separately and wraps 'extend_run' -/
@@ -754,9 +543,123 @@ lemma make_run_sprint_mem_journey_cell_close (D : Devil) (p n : Nat) (ppos : 0 <
   · convert hmem
     exact Nat.sub_one_add_one inz
 
--- The 'make_run' journey is "allowed" if the devil is "nice".
--- That is, it never visits an eaten cell.
--- TODO: Can we simplify this proof at all? It's rather lengthy.
+-- List of blocked cells used to generate 'next_sprint (make_run D p n ppos)'
+def make_block_list (D : Devil) (p n : Nat) (ppos : 0 < p) : List (Int × Int) :=
+  List.union (make_run D p n ppos).eaten (west_wall p (make_run D p n ppos).eaten.length)
+
+-- Expand the 'next_sprint' of a 'make_run' using 'make_block_list'
+lemma next_sprint_make_run_def (D : Devil) (p n : Nat) (ppos : 0 < p) :
+  next_sprint (make_run D p n ppos) =
+  sprint p (final_state (make_run D p n ppos)) (make_block_list D p n ppos) := rfl
+
+/- Note that it *is* possible to force the runner to remain on a blocked cell
+   if the devil is not nice. Technically, even with a devil that isn't nice,
+   the runner can never be forced onto a 'wall' cell (cells with x = -1, 0 ≤ y)
+   but that proof is more difficult and we're only concerned with nice devils
+   for this section of the proof so we can make our work easier by assuming such. -/
+lemma make_run_next_sprint_avoids_blocked_of_nice (D : Devil) (p n : Nat) (ppos : 0 < p) (hnice : nice D p) :
+  ∀ rs ∈ next_sprint (make_run D p n ppos), (loc rs) ∉ make_block_list D p n ppos := by
+  intro rs rsmem lrsmem
+  -- First handle the case where n = 0
+  -- This mostly involves showing that the origin will never be on the block list
+  by_cases nz : n = 0
+  · subst nz
+    apply sprint_avoids_blocked p _ (make_block_list D p 0 ppos) _ rs rsmem lrsmem
+    rw [make_run_eq_empty_of_length_zero]
+    rw [final_state_of_sprints_nil _ (empty_builder_sprints D p ppos)]
+    unfold run_start loc; dsimp
+    intro omem
+    -- We have two cases depending on whether rs is an eaten cell or wall cell
+    rcases List.mem_union_iff.mp omem with lhs | rhs
+    · -- The nice devil never eats the origin, so we can show a contradiction
+      rw [make_run_eq_empty_of_length_zero, empty_builder_eaten] at lhs
+      apply not_nice_of_eats_origin D p _ hnice
+      use NoSteps p, 0, (by rw [nosteps_steps p]; norm_num)
+      rw [List.mem_singleton.mp lhs]
+      rfl
+    · -- If rs is a wall cell, this leads to a contradiction because the
+      -- x-coordinates don't match
+      --rw [make_run_eaten_length, zero_add] at rhs
+      have := west_wall_xcoord_of_mem p _ (0, 0) rhs
+      dsimp at this
+      linarith
+  rename' nz => nnz; push_neg at nnz
+  have hsnnil : (make_run D p n ppos).sprints ≠ [] := by
+    apply List.ne_nil_of_length_pos
+    rw [make_run_sprints_length]
+    exact Nat.pos_of_ne_zero nnz
+  rw [next_sprint_make_run_def] at rsmem
+  -- Use recursion to show that the run has thus far avoided blocked cells
+  -- This will be required in order to use 'sprint_avoids_blocked'
+  have hsafe : loc (final_state (make_run D p n ppos)) ∉ make_block_list D p (n - 1) ppos := by
+    apply make_run_next_sprint_avoids_blocked_of_nice
+    · assumption
+    convert final_state_getLast_mem_of_nonnil (make_run D p n ppos) hsnnil
+    rw [List.getLast_congr _ _ (make_run_sprints_recurrence D p n ppos (Nat.pos_of_ne_zero nnz))]; swap
+    · apply List.append_ne_nil_of_right_ne_nil
+      exact list_singleton_ne_nil _
+    rw [List.getLast_append_right (list_singleton_ne_nil _)]
+    exact (List.getLast_singleton (list_singleton_ne_nil _)).symm
+  -- Strengthen the statement of 'hsafe' by including the devil's last response and
+  -- an extra 'p' cells in the west wall. This section constitutes the majority of the proof.
+  have hsafe' : loc (final_state (make_run D p n ppos)) ∉ make_block_list D p n ppos := by
+    intro lfsmem
+    rcases List.mem_union_iff.mp lfsmem with lhs | rhs
+    · -- Handle the case where the final state is on the 'eaten' list
+      rcases List.getElem_of_mem lhs with ⟨i, ilt, hi⟩
+      rw [make_run_eaten_length] at ilt
+      rw [getElem_congr_coll (make_run_eaten_recurrence D p n ppos (Nat.pos_of_ne_zero nnz))] at hi
+      -- Handle the case where the final state was eaten last
+      by_cases hin : i = n
+      · rw [List.getElem_append_right] at hi; swap
+        · rw [make_run_eaten_length, hin, Nat.sub_one_add_one nnz]
+        -- Prove a bound needed for 'getElem_singleton'
+        have lt1 : i - (make_run D p (n - 1) ppos).eaten.length < 1 := by
+          rw [make_run_eaten_length, Nat.sub_one_add_one nnz, hin, Nat.sub_self]
+          norm_num
+        rw [List.getElem_singleton lt1, final_state_loc_eq_journey_last] at hi
+        -- We will show that a journey cell is eaten, which is contradiction with 'hnice'
+        apply not_nice_of_eats_journey_cell D p _ hnice
+        use (make_run D p n ppos).A, n, n, le_refl n
+        use (by rw [make_run_journey_steps]; exact Nat.lt_add_one _)
+        have hsj := subjourney_full (make_run D p n ppos).A
+        rw [subjourney_congr_idx _ (make_run_journey_steps D p n ppos)] at hsj
+        rw [hsj]
+        convert hi
+        rw [last]
+        congr
+        rw [make_run_journey_steps]
+      · rename' hin => inen; push_neg at inen
+        -- If i ≠ n, we will show that the final state was on the old eaten list - a contradiction
+        apply hsafe
+        apply List.mem_union_iff.mpr; left
+        have ilt' : i < (make_run D p (n - 1) ppos).eaten.length := by
+          rw [make_run_eaten_length, Nat.sub_one_add_one nnz]
+          exact lt_of_le_of_ne (Nat.le_of_lt_add_one ilt) inen
+        rw [List.getElem_append_left ilt'] at hi
+        exact List.mem_of_getElem hi
+    · -- Now handle the case where the final state is a wall cell
+      unfold west_wall at rhs
+      rcases List.getElem_of_mem rhs with ⟨i, ilt, hi⟩
+      rw [List.length_map, List.length_range, make_run_eaten_length] at ilt
+      rw [List.getElem_map, final_state_loc_eq_journey_last] at hi
+      -- Handle the case where 'i' is so large, it exceeds the bound proven in Bound.lean
+      by_cases pni : p * n < i
+      · apply (lt_self_iff_false n).mp
+        nth_rw 2 [← make_run_journey_steps D p n ppos]
+        apply journey_lb _ _ (lt_of_lt_of_le pni (le_trans _ (le_max_right _ _)))
+        simp
+        rw [← (Prod.ext_iff.mp hi).2, List.getElem_range]
+        exact (le_refl i)
+      rename' pni => ilepn; push_neg at ilepn
+      · -- If i ≤ p * n, show that the final state was in the old west wall
+        apply hsafe (List.mem_union_iff.mpr _); right
+        rw [List.getElem_range] at hi
+        rw [final_state_loc_eq_journey_last, ← hi]
+        apply west_wall_mem
+        rwa [make_run_eaten_length, Nat.sub_one_add_one nnz]
+  exact sprint_avoids_blocked p _ _ hsafe' rs rsmem lrsmem
+
 lemma make_run_journey_allowed_of_nice (D : Devil) (p n : Nat) (ppos : 0 < p) (hnice : nice D p) :
   allowed D (make_run D p n ppos).A := by
   let MR := make_run D p n ppos
@@ -778,11 +681,10 @@ lemma make_run_journey_allowed_of_nice (D : Devil) (p n : Nat) (ppos : 0 < p) (h
     ) := by
     rw [subjourney_congr_journey (make_run_journey_recurrence D p n ppos npos)]
     rw [append_subjourney]
-  rw [lhs_rw]
   -- If j ≠ n we can recurse, so handle that case first
   by_cases hjnn : n ≠ j
   · -- Now apply the journey recurrence on the right and recurse
-    rw [cell_congr_journey (make_run_journey_recurrence D p n ppos npos)]
+    rw [lhs_rw, cell_congr_journey (make_run_journey_recurrence D p n ppos npos)]
     rw [append_cell_ne_last]; swap
     · rw [make_run_journey_steps, Nat.sub_one_add_one nnez]
       exact lt_of_le_of_ne (Nat.le_of_lt_add_one jlt') hjnn.symm
@@ -791,60 +693,42 @@ lemma make_run_journey_allowed_of_nice (D : Devil) (p n : Nat) (ppos : 0 < p) (h
     · exact ilt
   rename' hjnn => hjn; push_neg at hjn
   subst hjn
-  -- Now we can also use recursion and the fact that the devil is nice
-  -- to prove that the second-to-last cell in the journey is not in
-  -- the eaten list.
-  let MR' := (make_run D p (n - 1) ppos)
-  let rs₀ := final_state MR'
-  have : loc rs₀ ∉ MR'.eaten := by
-    intro h
-    rcases List.getElem_of_mem h with ⟨k, klt, h⟩
-    rw [make_run_eaten_length] at klt
-    rw [make_run_eaten] at h; swap
-    · assumption
-    rw [← make_run_subjourney D p k (n - 1) ppos] at h; swap
-    · assumption
-    unfold rs₀ at h
-    rw [final_state_loc_eq_journey_last, last] at h
-    rw [cell_congr_idx MR'.A (make_run_journey_steps D p (n - 1) ppos)] at h
-    -- Show that k < n - 1 or else D is not "nice" - a contradiction
-    have klt' : k < n - 1 := by
-      apply lt_of_le_of_ne (Nat.le_of_lt_add_one klt)
-      contrapose! hnice
-      subst hnice
-      apply not_nice_of_eats_journey_cell
-      use MR'.A, (n - 1), (n - 1), le_rfl, (by
-        rw [make_run_journey_steps, Nat.sub_one_add_one nnez]
-        exact Nat.sub_one_lt nnez
-      )
-    -- Now recurse
-    apply make_run_journey_allowed_of_nice D p (n - 1) ppos hnice _ _ klt' _ h
-  -- Rewrite the left-hand_side as an element of the 'eaten' list
-  rw [make_run_subjourney, ← make_run_eaten D p n]
-  -- Resolve bounds checks first
-  pick_goal 2; pick_goal 3
-  · rwa [Nat.sub_one_add_one nnez]
-  · exact lt_trans ilt (Nat.lt_add_one _)
-  -- Re-write the right-hand side so that we can apply 'sprint_avoids_eaten'
-  have nplt : n - 1 < n := Nat.sub_lt npos (by norm_num)
-  have nplt' : n - 1 < MR.sprints.length := by rwa [make_run_sprints_length]
-  have rhs_rw : cell MR.A n jlt =
-    loc (((make_run D p n ppos).sprints[n - 1]'nplt').getLast
-      (MR.nonnil _ (List.getElem_mem _))) := by
-    rw [cell_congr_idx _ (Nat.sub_one_add_one nnez).symm]
-    exact make_run_journey_cell D p n ppos (n - 1) nplt
-  rw [rhs_rw]
-  -- Apply the eaten recurrence
-  rw [getElem_congr_coll (make_run_eaten_recurrence D p n ppos npos)]
-  rw [List.getElem_append_left]; swap
-  · -- Resolve bounds check
-    rwa [make_run_eaten_length, Nat.sub_one_add_one nnez]
-  by_contra! h
-  -- Finally, apply 'sprint_avoids_eaten' which states that a sprint never
-  -- visits a cell from the eaten list used to create it.
-  apply sprint_avoids_eaten p rs₀ MR'.eaten this _ _ (List.mem_of_getElem h)
-  rw [List.getLast_congr _ (next_sprint_nonnil _) (make_run_sprint D p n ppos (n - 1) nplt)]
-  exact List.getLast_mem (next_sprint_nonnil _)
+  have last_exp := (final_state_loc_eq_journey_last (make_run D p n ppos)).symm
+  rw [last, ← cell_congr_idx _ (make_run_journey_steps D p n ppos).symm jlt] at last_exp
+  rw [last_exp, make_run_subjourney D p i n ppos (lt_trans ilt (Nat.lt_add_one _))]
+  intro h
+  let fs : RunState := final_state (make_run D p n ppos)
+  have lfsmem : loc fs ∈ (make_run D p (n - 1) ppos).eaten := by
+    apply @List.mem_of_mem_take _ (i + 1)
+    rw [make_run_eaten_take]; swap
+    · rwa [Nat.sub_one_add_one nnez]
+    -- Handle the case where i = 0
+    by_cases iz : i = 0
+    · subst iz
+      rw [make_run_eq_empty_of_length_zero] at *
+      rw [empty_builder_journey] at h
+      rw [empty_builder_eaten, h]
+      exact List.mem_singleton_self _
+    rename' iz => inz; push_neg at inz
+    -- Otherwise, if i ≠ 0 we can use the 'eaten' recurrence
+    rw [make_run_eaten_recurrence]; swap
+    · exact Nat.pos_of_ne_zero inz
+    apply List.mem_append_right
+    rw [h]
+    exact List.mem_singleton_self _
+  apply make_run_next_sprint_avoids_blocked_of_nice D p (n - 1) ppos hnice fs _ _
+  · convert final_state_getLast_mem_of_nonnil (make_run D p n ppos) (by
+      apply List.ne_nil_of_length_pos
+      rwa [make_run_sprints_length]
+    )
+    rw [List.getLast_congr _ _ (make_run_sprints_recurrence D p n ppos npos)]; swap
+    · apply List.ne_nil_of_length_pos
+      rw [List.length_append, List.length_singleton]
+      exact lt_of_le_of_lt (Nat.zero_le _) (Nat.lt_add_one _)
+    rw [List.getLast_append_right]; swap
+    · exact list_singleton_ne_nil _
+    exact (List.getLast_singleton (list_singleton_ne_nil _)).symm
+  · exact List.mem_union_iff.mpr (Or.inl lfsmem)
 
 /- Construct the list of run states corresponding to the full route of the runner.
    Each sprint overlaps by one cell, so we need to remove the first state from all
@@ -1039,33 +923,12 @@ lemma make_run_runner_avoids_eaten_cells_of_nice (D : Devil) (p n : Nat) (ppos :
   rw [lhs_rw]
   rw [getElem_congr_coll (make_run_eaten_take D p i n ppos (lt_trans ilt (Nat.lt_add_one _)))]
   intro h
-  let MR := (make_run D p i ppos)
-  let rs₀ := final_state MR
-  -- TODO: There is a very similar section in 'make_run_journey_allowed_of_nice'
-  -- Can we refactor this into a separate proof somehow?
-  have hsafe : loc rs₀ ∉ MR.eaten := by
-    intro h
-    rcases List.getElem_of_mem h with ⟨l, llt, h⟩
-    rw [make_run_eaten_length] at llt
-    rw [final_state_loc_eq_journey_last, last, make_run_eaten] at h; swap
-    · exact llt
-    rw [← make_run_subjourney D p l i] at h; swap
-    · exact llt
-    rw [cell_congr_idx _ (make_run_journey_steps D p i ppos)] at h
-    -- Handle the case where l = i using 'not_nice_of_eats_journey_cell'
-    by_cases hli : l = i
-    · subst hli
-      absurd hnice
-      apply not_nice_of_eats_journey_cell
-      use MR.A, l, l, le_rfl, (by rwa [make_run_journey_steps])
-    rename' hli => lnei; push_neg at lnei
-    -- Resolve the goal with 'make_run_journey_allowed_of_nice
-    absurd h
-    apply make_run_journey_allowed_of_nice
-    · exact hnice
-    · exact lt_of_le_of_ne (Nat.le_of_lt_add_one llt) lnei
-  -- Use 'sprint_avoids_eaten' with the above sub-result to get a contradiction
-  apply sprint_avoids_eaten p rs₀ MR.eaten hsafe _ (List.getElem_mem _) (List.mem_of_getElem h)
+  rw [make_run_sprint D p n ppos i ilt] at jlt
+  let rs : RunState := (next_sprint (make_run D p i ppos))[j]'jlt
+  apply make_run_next_sprint_avoids_blocked_of_nice D p i ppos hnice rs (List.getElem_mem jlt)
+  apply List.mem_union_iff.mpr; left
+  rw [← h]
+  exact List.getElem_mem (by rw [make_run_eaten_length]; exact Nat.lt_add_one_of_le kle)
 
 -- If the devil is "nice", then no cell visited by the runner was ever eaten by the devil.
 lemma run_path_not_eaten_of_nice (D : Devil) (p n : Nat) (ppos : 0 < p) (hnice : nice D p) :
