AngelDevil/Sprint.lean
@@ -1,0 +1,163 @@
+import Mathlib.Tactic.NormNum.Core
+import Mathlib.Tactic.Contrapose
+import AngelDevil.Basic
+import AngelDevil.Util
+import AngelDevil.Trace
+
+set_option linter.style.longLine false
+
+-- A useful equivalence for the following definitions / lemmas
+lemma sprint_fin_prop (p : Nat) (start : RunState) (blocked : List (Int × Int)) (ppos : 0 < p) :
+  ∀ i, i < (trace (2 * p) start blocked).length ↔ i < 2 * p - 1 + 1 := by
+  intro i
+  constructor
+  · intro h
+    rw [Nat.sub_one_add_one]; swap
+    · apply Nat.ne_zero_of_lt
+      exact (Nat.mul_lt_mul_left (two_pos)).mpr ppos
+    rwa [trace_length] at h
+  · intro h
+    rw [trace_length]
+    rwa [Nat.sub_one_add_one] at h
+    apply Nat.ne_zero_iff_zero_lt.mpr
+    exact Nat.mul_pos two_pos ppos
+
+abbrev sprint_end_fun (p : Nat) (start : RunState) (blocked : List (Int × Int)) (ppos : 0 < p) :
+  Fin (2 * p - 1 + 1) → Prop := fun i ↦ ¬close p (loc start) (loc ((trace (2 * p) start blocked)[i]'(by
+    rw [sprint_fin_prop]
+    · exact i.2
+    · assumption
+  )))
+
+-- Define a "sprint" as the trace with length no greater than '2p' for which every
+-- cell in the trace is "close" to the start.
+def sprint (p : Nat) (start : RunState) (blocked : List (Int × Int)) : List RunState :=
+  trace (if h : (∃ rs : RunState, rs ∈ trace (2 * p) start blocked ∧ ¬close p (loc start) (loc rs)) then
+  (_find_first (sprint_end_fun p start blocked (by
+    rcases h with ⟨rs, h₀, h₁⟩
+    have ppos := List.length_pos_of_mem h₀
+    rw [trace_length] at ppos
+    exact Nat.pos_of_mul_pos_left ppos
+  ))) else (2 * p)) start blocked
+
+lemma sprint_getElem_zero_of_nonnil (p : Nat) (start : RunState) (blocked : List (Int × Int)) :
+  (hnnil : sprint p start blocked ≠ []) →
+  (sprint p start blocked)[0]'(List.length_pos_iff.mpr hnnil) = start := by
+  intro hnnil
+  unfold sprint
+  apply trace_getElem_zero_of_nonnil
+  exact hnnil
+
+-- If 'p' is positive, the sprint will not be empty
+lemma sprint_nonnil_of_ppos (p : Nat) (start : RunState) (blocked : List (Int × Int)) :
+  0 < p → sprint p start blocked ≠ [] := by
+  intro ppos
+  apply List.ne_nil_of_length_pos
+  rw [sprint, trace_length]
+  split_ifs with h
+  · rcases h with ⟨rs, h₀, h₁⟩
+    apply Nat.pos_of_ne_zero
+    intro hfind
+    have : sprint_end_fun p start blocked ppos 0 := by
+      rw [← Fin.val_eq_zero_iff.mp hfind]
+      apply _find_first_is_sat
+      rcases List.getElem_of_mem h₀ with ⟨i, ilt, hirs⟩
+      let i' : Fin (2 * p - 1 + 1) := ⟨i, (sprint_fin_prop p start blocked ppos i).mp ilt⟩
+      use i'
+      unfold sprint_end_fun
+      rw [← hirs] at h₁
+      exact h₁
+    apply this
+    convert close_self p (loc start)
+    apply trace_getElem_zero_of_nonnil
+    apply List.ne_nil_of_length_pos
+    rw [trace_length]
+    exact Nat.mul_pos two_pos ppos
+  exact Nat.mul_pos (by norm_num) ppos
+
+lemma sprint_getElem_zero_of_ppos (p : Nat) (start : RunState) (blocked : List (Int × Int)) :
+  (ppos : 0 < p) → (sprint p start blocked)[0]'(by
+    apply List.length_pos_of_ne_nil
+    exact sprint_nonnil_of_ppos p start blocked ppos
+  ) = start :=
+  fun ppos ↦
+  sprint_getElem_zero_of_nonnil p start blocked (sprint_nonnil_of_ppos p start blocked ppos)
+
+-- The maximum sprint length is 2 * p
+lemma sprint_length_le (p : Nat) (start : RunState) (blocked : List (Int × Int)) :
+  (sprint p start blocked).length ≤ 2 * p := by
+  unfold sprint
+  rw [trace_length]
+  split_ifs with h; swap
+  · rfl
+  rcases h with ⟨rs, hmem, hnclose⟩
+  rcases List.getElem_of_mem hmem with ⟨i, ilt, hirs⟩
+  apply le_of_lt (lt_of_lt_of_le (Fin.prop _) _)
+  rw [Nat.sub_one_add_one]
+  rw [trace_length] at ilt
+  apply Nat.ne_zero_of_lt ilt
+
+-- Each run state in a sprint is equal to the corresponding element of the corresponding trace
+lemma sprint_getElem_eq_trace_getElem (p : Nat) (start : RunState) (blocked : List (Int × Int)) :
+  ∀ i (ilt : i < (sprint p start blocked).length),
+  (sprint p start blocked)[i] = (trace (2 * p) start blocked)[i]'(by
+    rw [trace_length]
+    exact lt_of_lt_of_le ilt (sprint_length_le p start blocked)
+  ) := by
+  intro i ilt
+  have twoppos : 0 < (2 * p) := by
+    apply lt_of_le_of_lt (Nat.zero_le _)
+    exact (lt_of_lt_of_le ilt (sprint_length_le p start blocked))
+  unfold sprint
+  split_ifs with h
+  · rw [getElem_congr_coll (trace_take (2 * p) start blocked _ _)]; swap
+    · apply le_of_lt
+      nth_rw 14 [← Nat.sub_one_add_one (Nat.ne_zero_of_lt twoppos)]
+      exact Fin.prop _
+    apply List.getElem_take
+  rfl
+
+-- All run states in a sprint are close to the start of that sprint
+lemma sprint_close_mem_head (p : Nat) (ppos : 0 < p) (start : RunState) (blocked : List (Int × Int)) :
+  ∀ x ∈ (sprint p start blocked), close p (loc x)
+  (loc ((sprint p start blocked).head (sprint_nonnil_of_ppos p start blocked ppos))) := by
+  intro x hmem
+  rw [← List.getElem_zero_eq_head]; swap
+  · exact List.length_pos_of_mem hmem
+  rw [sprint_getElem_zero_of_nonnil, close_comm]; swap
+  · exact List.ne_nil_of_mem hmem
+  rcases List.getElem_of_mem hmem with ⟨i, ilt, rfl⟩
+  rw [sprint_getElem_eq_trace_getElem p start blocked i ilt]
+  by_contra! h
+  have ilt' := lt_of_lt_of_le ilt (sprint_length_le p start blocked)
+  have ppos : 0 < p := by
+    apply (Nat.mul_lt_mul_left (two_pos)).mp
+    rw [mul_zero]
+    exact lt_of_le_of_lt (Nat.zero_le _) ilt'
+  let i' : Fin (2 * p - 1 + 1) := ⟨i, lt_of_lt_of_eq ilt' (Nat.sub_one_add_one (Nat.ne_zero_of_lt ilt')).symm⟩
+  unfold sprint at ilt
+  have hthen : ∃ rs ∈ trace (2 * p) start blocked, ¬close p (loc start) (loc rs) := by
+    use (trace (2 * p) start blocked)[i]'(by rwa [trace_length])
+    use List.getElem_mem (by rwa [trace_length])
+  rw [dif_pos hthen, trace_length] at ilt
+  have := _find_first_is_first (sprint_end_fun p start blocked ppos) i' h
+  exact Nat.not_lt.mpr this ilt
+
+-- Prove that the first and last cells in a sprint are "close"
+lemma sprint_close_first_last (p : Nat) (hpos : 0 < p) (start : RunState) (blocked : List (Int × Int)) :
+  close p
+  (loc ((sprint p start blocked).head (sprint_nonnil_of_ppos p start blocked hpos)))
+  (loc ((sprint p start blocked).getLast (sprint_nonnil_of_ppos p start blocked hpos))) := by
+  have hnnil := sprint_nonnil_of_ppos p start blocked hpos
+  rw [close_comm]
+  exact sprint_close_mem_head p hpos start blocked _ (List.getLast_mem hnnil)
+
+-- The runner never visits an eaten cell
+-- (as long as they don't start on an eaten cell)
+lemma sprint_avoids_blocked (p : Nat) (start : RunState)
+  (blocked : List (Int × Int)) (hsafe : loc start ∉ blocked) :
+  ∀ x, x ∈ (sprint p start blocked) → loc x ∉ blocked := by
+  intro x hmem₀ hmem₁
+  unfold sprint at hmem₀
+  split_ifs at hmem₀ with h
+  repeat exact trace_avoids_blocked _ start blocked hsafe x hmem₀ hmem₁
